cedar-lean/Cedar/Thm/Data/Map.lean
@@ -27,12 +27,40 @@ This file proves useful properties of canonical list-based maps defined in
 
 namespace Cedar.Data.Map
 
-/-! ### Well-formed sets -/
+/-! ### Well-formed maps -/
 
 def WellFormed {α β} [LT α] [DecidableLT α] (m : Map α β) :=
   m = Map.make m.toList
 
-/-! ### contains and mem -/
+/-
+  In well-formed maps, if there are two pairs with the same key, then they have
+  the same value
+-/
+theorem key_maps_to_one_value [BEq α] [LT α] [DecidableLT α] (k : α) (v₁ v₂ : β) (m : Map α β) :
+  m.WellFormed →
+  (k, v₁) ∈ m.kvs →
+  (k, v₂) ∈ m.kvs →
+  v₁ = v₂
+:= by
+  unfold WellFormed toList
+  intro wf h₁ h₂
+  sorry
+
+/-
+  In well-formed maps, if a key maps to a value, then all equal keys (by BEq)
+  also map to that value
+-/
+theorem equal_keys_same_value [BEq α] [LT α] [DecidableLT α] (k₁ k₂ : α) (v : β) (m : Map α β) :
+  m.WellFormed →
+  (k₁, v) ∈ m.kvs →
+  k₁ == k₂ →
+  (k₂, v) ∈ m.kvs
+:= by
+  unfold WellFormed toList
+  intro wf h₁ h₂
+  sorry
+
+/-! ### contains, mem, and find? -/
 
 theorem in_list_in_map {α : Type u} (k : α) (v : β) (m : Map α β) :
   (k, v) ∈ m.kvs → k ∈ m
@@ -41,6 +69,62 @@ theorem in_list_in_map {α : Type u} (k : α) (v : β) (m : Map α β) :
   have h₁ : k ∈ (List.map Prod.fst m.kvs) := by simp only [List.mem_map] ; exists (k, v)
   apply h₁
 
+theorem in_list_some_find? [DecidableEq α] [LT α] [DecidableLT α] (k : α) (v : β) (m : Map α β) :
+  m.WellFormed →
+  ((k, v) ∈ m.kvs ↔ m.find? k = some v)
+:= by
+  intro h₁
+  unfold find?
+  constructor
+  case mp =>
+    intro h₂
+    cases h₃ : m.kvs.find? λ x => match x with | (k', _) => k' == k
+    case none =>
+      exfalso
+      rw [List.find?_eq_none] at h₃
+      specialize h₃ (k, v) h₂
+      apply h₃ ; clear h₃
+      simp
+    case some kv =>
+      simp
+      have h₄ := List.find?_some h₃
+      simp at h₄
+      subst h₄
+      replace h₃ := List.mem_of_find?_eq_some h₃
+      apply (key_maps_to_one_value kv.fst v kv.snd m h₁ h₂ _).symm
+      trivial
+  case mpr =>
+    intro h₂
+    cases h₃ : m.kvs.find? λ x => match x with | (k', _) => k' == k
+    case none => simp [h₃] at h₂
+    case some kv =>
+      simp [h₃] at h₂
+      subst h₂
+      have h₄ := List.mem_of_find?_eq_some h₃
+      replace h₃ := List.find?_some h₃
+      split at h₃ ; rename_i k' v
+      simp
+      exact equal_keys_same_value k' k v m h₁ h₄ h₃
+
+/- currently unused -/
+/-
+theorem contains_iff_in_map [BEq α] (k : α) (m : Map α β) :
+  m.contains k ↔ k ∈ m
+:= by
+  simp [contains, Option.isSome_iff_exists]
+  constructor
+  case mp =>
+    simp [find?]
+    intro v h₁
+    apply in_list_in_map k v m
+    split at h₁ <;> simp at h₁
+    subst h₁
+    case h_1 k' v h₁ =>
+      have h₂ := List.mem_of_find?_eq_some h₁ ; simp at h₂
+      have h₃ := List.find?_some h₁ ; simp at h₃
+      simp [h₃] at h₂
+-/
+
 theorem contains_iff_some_find? {α β} [BEq α] {m : Map α β} {k : α} :
   m.contains k ↔ ∃ v, m.find? k = .some v
 := by simp [contains, Option.isSome_iff_exists]
@@ -48,6 +132,27 @@ theorem contains_iff_some_find? {α β} [BEq α] {m : Map α β} {k : α} :
 theorem not_contains_of_empty {α β} [BEq α] (k : α) :
   ¬ (Map.empty : Map α β).contains k
 := by simp [contains, empty, find?, List.find?]
+
+theorem in_values_iff_some_find? {α β} [DecidableEq α] [LT α] [DecidableLT α] {m : Map α β} {v : β} :
+  m.WellFormed →
+  (v ∈ m.values ↔ ∃ k, m.find? k = .some v)
+:= by
+  simp [values]
+  intro wf
+  constructor
+  case mp =>
+    intro h₁
+    replace ⟨⟨k, v'⟩, ⟨h₁, h₂⟩⟩ := h₁
+    exists k
+    simp [Prod.snd] at h₂
+    subst v'
+    rw [← in_list_some_find? k v m wf]
+    trivial
+  case mpr =>
+    intro h₁
+    replace ⟨k, h₁⟩ := h₁
+    rw [← in_list_some_find? k v m wf] at h₁
+    exists (k, v)
 
 /-! ### make -/
 
@@ -70,6 +175,12 @@ theorem make_nil_is_empty {α β} [LT α] [DecidableLT α] :
 := by simp [make, empty, List.canonicalize_nil]
 
 /-! ### find? and mapOnValues -/
+
+theorem mapOnValues_wf [LT α] [DecidableLT α] [DecidableEq α] {f : β → γ} {m : Map α β} :
+  m.WellFormed ↔ (m.mapOnValues f).WellFormed
+:= by
+  unfold mapOnValues WellFormed
+  sorry
 
 theorem find?_mapOnValues {α β γ} [LT α] [DecidableLT α] [DecidableEq α] (f : β → γ) (m : Map α β) (k : α)  :
   (m.find? k).map f = (m.mapOnValues f).find? k
@@ -95,26 +206,14 @@ theorem find?_mapOnValues_none {α β γ} [LT α] [DecidableLT α] [DecidableEq 
   simp [Option.map, h₁]
 
 theorem mapOnValues_eq_make_map {α β γ} [LT α] [StrictLT α] [DecidableLT α] (f : β → γ) {m : Map α β}
-  (h₁ : m.WellFormed) :
+  (wf : m.WellFormed) :
   m.mapOnValues f = Map.make (m.toList.map λ kv => (kv.fst, f kv.snd))
 := by
-  simp [Map.WellFormed] at h₁
-  simp [Map.mapOnValues, Map.toList, Map.kvs, Map.make] at *
-  rw [h₁] ; simp only ; rw [eq_comm]
-  have h₂ : Prod.map id f = (fun (x : α × β) => (x.fst, f x.snd)) := by unfold Prod.map ; simp only [id_eq]
-  simp only [← h₂, ← List.canonicalize_of_map_fst, List.canonicalize_idempotent]
-
-theorem find?_mem_toList {α β} [LT α] [DecidableLT α] [DecidableEq α] {m : Map α β} {k : α} {v : β}
-  (h₁ : m.find? k = .some v) :
-  (k, v) ∈ m.toList
-:= by
-  simp [Map.toList, Map.kvs, Map.find?] at *
-  split at h₁ <;> simp at h₁
-  subst h₁
-  rename_i h₂
-  have h₃ := List.find?_some h₂
-  simp at h₃ ; subst h₃
-  exact List.mem_of_find?_eq_some h₂
+  unfold WellFormed at wf
+  simp [mapOnValues, toList, kvs, make] at *
+  rw [wf] ; simp only ; rw [eq_comm]
+  have h₁ : Prod.map id f = (fun (x : α × β) => (x.fst, f x.snd)) := by unfold Prod.map ; simp only [id_eq]
+  simp only [← h₁, ← List.canonicalize_of_map_fst, List.canonicalize_idempotent]
 
 theorem mapOnValues_contains {α β γ} [LT α] [DecidableLT α] [DecidableEq α] (f : β → γ) {m : Map α β} {k : α} :
   Map.contains m k = Map.contains (Map.mapOnValues f m) k
@@ -124,36 +223,58 @@ theorem mapOnValues_contains {α β γ} [LT α] [DecidableLT α] [DecidableEq α
   case h_1 h => simp [find?_mapOnValues_some f h]
   case h_2 h => simp [find?_mapOnValues_none f h]
 
-theorem findOrErr_mapOnValues [LT α] [DecidableLT α] [BEq α] [DecidableEq α] {f : β → γ} {m : Map α β} {k : α} {e : Error} :
+theorem values_mapOnValues [LT α] [StrictLT α] [DecidableLT α] [DecidableEq α] (f : β → γ) {m : Map α β} :
+  (m.mapOnValues f).values = m.values.map f
+:= by
+  unfold mapOnValues values
+  simp [kvs]
+  repeat rw [← List.map_map]
+  induction m.1
+  case nil => simp
+  case cons kv tail h_ind =>
+    simp [List.map_cons]
+    repeat rw [← List.map_map]
+    trivial
+
+theorem findOrErr_mapOnValues [LT α] [DecidableLT α] [DecidableEq α] {f : β → γ} {m : Map α β} {k : α} {e : Error} :
   (m.mapOnValues f).findOrErr k e = (m.findOrErr k e).map f
 := by
   unfold findOrErr
-  split <;> simp [Except.map]
-  case h_1 v h₁ =>
-    rename_i inst1 inst2 inst3 inst4 _
-    have h₂ := @find?_mapOnValues α β γ inst1 inst2 inst4 f m k
-    rw [eq_comm] at h₂
-    simp [h₁] at h₂
-    rw [h₂] at h₁
+  rw [← find?_mapOnValues]
+  cases m.find? k <;> simp [Except.map]
 
+theorem findOrErr_ok_iff_find?_some [LT α] [DecidableLT α] [DecidableEq α] {m : Map α β} {k : α} {v : β} {e : Error} :
+  m.findOrErr k e = .ok v ↔ m.find? k = some v
+:= by
+  unfold findOrErr
+  cases m.find? k <;> simp
 
-  have h₁ := find?_mapOnValues f m k
-  simp [← h₁]
-  rw [← find?_mapOnValues f m k]
+theorem in_values_iff_findOrErr_ok [LT α] [DecidableLT α] [DecidableEq α] {m : Map α β} {v : β} {e : Error}
+  (wf : m.WellFormed) :
+  v ∈ m.values ↔ ∃ k, m.findOrErr k e = .ok v
+:= by
+  simp [values, findOrErr_ok_iff_find?_some]
+  constructor
+  case mp =>
+    intro h₁
+    replace ⟨⟨k, v'⟩, ⟨h₁, h₂⟩⟩ := h₁
+    simp at h₂
+    subst v'
+    exists k
+    simp [← in_list_some_find? k v m wf]
+    trivial
+  case mpr =>
+    intro h₁
+    replace ⟨k, h₁⟩ := h₁
+    exists (k, v)
+    simp [in_list_some_find? k v m wf]
+    trivial
 
 /- not currently needed -/
 theorem mapM_on_kvs_eqv_mapM_on_map [LT α] [DecidableLT α] (f : β → Option γ) {m : Map α β} :
   (m.kvs.mapM λ x => f x.snd) = (m.mapMOnValues f).map Map.values
 := by
   sorry
-
-/-
-theorem something [LT α] [DecidableLT α] (f : β → γ) (g : α × γ → Option ψ) {m : Map α β} :
-  (m.mapOnValues f).kvs.mapM g = m.mapMOnValues (f ∘ g)
-:= by
-  sorry
--/
-
 
 /-! ### sizeOf -/
 
