cedar-lean/Cedar/Thm/PartialEval/GetAttr.lean
@@ -54,13 +54,110 @@ theorem lhs_unknown {x₁ : PartialExpr} {attr : String} :
   case right => exact h₁.right
 
 /--
+  helper lemma: if a `RestrictedPartialExpr` is an unknown, then it's still an
+  unknown after converting it to `PartialExpr`
+-/
+theorem restrictedPartialExpr_to_PartialExpr_preserves_isUnknown {rpexpr : RestrictedPartialExpr} :
+  rpexpr.isUnknown → rpexpr.asPartialExpr.isUnknown
+:= by
+  unfold RestrictedPartialExpr.isUnknown PartialExpr.isUnknown RestrictedPartialExpr.asPartialExpr
+  cases rpexpr <;> simp
+
+/--
+  helper lemma: if a `RestrictedPartialExpr` contains an unknown, then it still does
+  after converting it to `PartialExpr`
+-/
+theorem restrictedPartialExpr_to_PartialExpr_preserves_containsUnknown {rpexpr : RestrictedPartialExpr} :
+  rpexpr.containsUnknown → rpexpr.asPartialExpr.containsUnknown
+:= by
+  unfold RestrictedPartialExpr.containsUnknown PartialExpr.containsUnknown
+  cases rpexpr <;> simp
+  case lit | call =>
+    intro x h₁ h₂
+    simp [RestrictedPartialExpr.subexpressions] at h₁
+    subst h₁
+    simp [RestrictedPartialExpr.isUnknown] at h₂
+  case unknown name =>
+    intro x h₁ h₂
+    simp [RestrictedPartialExpr.subexpressions] at h₁
+    subst h₁
+    exists (.unknown name)
+    simp [PartialExpr.isUnknown, RestrictedPartialExpr.asPartialExpr, PartialExpr.subexpressions]
+  case set xs | record attrs =>
+    intro x h₁ h₂
+    simp [RestrictedPartialExpr.subexpressions] at h₁
+    rcases h₁ with h₁ | h₁
+    case inl =>
+      subst h₁
+      simp [RestrictedPartialExpr.isUnknown] at h₂
+    case inr =>
+      -- `rpexpr` is a set or record that recursively contains an unknown
+      exists x.asPartialExpr
+      unfold RestrictedPartialExpr.asPartialExpr PartialExpr.subexpressions
+      cases x <;> simp [RestrictedPartialExpr.isUnknown] at h₂
+      case unknown name =>
+        split <;> simp <;> rename_i h₃ <;> simp at h₃
+        case h_5 name' =>
+          subst h₃
+          simp [PartialExpr.isUnknown]
+          sorry
+
+/--
+  if `entities.attrs uid` is `ok` with some attrs, those attrs are a
+  well-formed `Map`
+-/
+theorem partialEntities_attrs_wf {entities : PartialEntities} {uid : EntityUID} {attrs: Map String RestrictedPartialValue} :
+  entities.AllWellFormed →
+  entities.attrs uid = ok attrs →
+  attrs.WellFormed
+:= by
+  unfold PartialEntities.attrs PartialEntities.AllWellFormed PartialEntityData.WellFormed
+  intro wf h₁
+  cases h₂ : entities.findOrErr uid Error.entityDoesNotExist <;> simp [h₂] at h₁
+  case ok attrs =>
+    subst h₁
+    have ⟨wf_m, wf_edata⟩ := wf ; clear wf
+    apply (wf_edata _ _).left
+    have h₃ := Map.in_values_iff_findOrErr_ok (v := attrs) (e := Error.entityDoesNotExist) wf_m
+    simp [h₃]
+    exists uid
+
+/--
+  if `partialAttrsOf` returns `ok` with some attrs, those attrs are a
+  well-formed `Map`
+-/
+theorem partialAttrsOf_wf {entities : PartialEntities} {v : Value} {attrs : Map String RestrictedPartialValue} :
+  entities.AllWellFormed →
+  v.WellFormed →
+  partialAttrsOf v entities.attrs = ok attrs →
+  attrs.WellFormed
+:= by
+  intro wf_e wf_v
+  unfold partialAttrsOf
+  cases v <;> try simp
+  case prim p =>
+    cases p <;> simp
+    case entityUID uid => exact partialEntities_attrs_wf wf_e
+  case record r =>
+    intro h₁
+    subst h₁
+    apply Map.mapOnValues_wf.mp wf_v
+
+/--
   `partialAttrsOf` on concrete arguments is the same as `attrsOf` on those
   arguments
 -/
 theorem partialAttrsOf_on_concrete_eqv_attrsOf {v : Value} {entities : Entities} :
   partialAttrsOf v (PartialEntities.attrs entities) = (attrsOf v (Entities.attrs entities)).map λ m => m.mapOnValues RestrictedPartialValue.value
 := by
-  sorry
+  unfold partialAttrsOf attrsOf Except.map
+  cases v <;> simp
+  case prim p =>
+    cases p <;> simp
+    case entityUID uid =>
+      unfold PartialEntities.attrs Entities.attrs Entities.asPartialEntities
+      cases h₁ : entities.findOrErr uid Error.entityDoesNotExist
+      <;> simp [h₁, Map.findOrErr_mapOnValues, Except.map, EntityData.asPartialEntityData]
 
 /--
   `partialGetAttr` on concrete arguments is the same as `getAttr` on those
@@ -73,6 +170,49 @@ theorem partialGetAttr_on_concrete_eqv_getAttr {v₁ : Value} {entities : Entiti
   simp [partialAttrsOf_on_concrete_eqv_attrsOf, Except.map]
   cases h₁ : attrsOf v₁ entities.attrs <;> simp
   case ok m => simp [Map.findOrErr_mapOnValues, Except.map]
+
+/--
+  helper lemma:
+
+  If `ResidualsContainUnknowns` is true for an `Entities`, and `partialAttrsOf`
+  returns `ok`, then `ResidualsContainUnknowns` is also true for all the
+  attributes returned by `partialAttrsOf`
+-/
+theorem partialAttrsOf_ResidualsContainUnknowns {entities : PartialEntities} {v : Value} :
+  entities.WellFormed →
+  PartialEntities.ResidualsContainUnknowns entities →
+  partialAttrsOf v entities.attrs = .ok attrs →
+  ∀ rpval ∈ attrs.values, RestrictedPartialValue.ResidualsContainUnknowns rpval
+:= by
+  unfold PartialEntities.ResidualsContainUnknowns partialAttrsOf
+  intro wf h₁ h₂ rpval h₃
+  split at h₂
+  case h_1 attrs' =>
+    simp at h₂
+    subst h₂
+    unfold RestrictedPartialValue.ResidualsContainUnknowns
+    split <;> try simp
+    case h_1 r =>
+      exfalso
+      rw [Map.values_mapOnValues] at h₃
+      generalize attrs'.values = vs at h₃
+      induction vs
+      case nil => simp at h₃
+      case cons h_ind =>
+        apply h_ind ; clear h_ind
+        unfold List.map at h₃
+        simp [List.mem_cons] at h₃
+  case h_2 uid =>
+    unfold PartialEntities.attrs at h₂
+    cases h₄ : entities.findOrErr uid Error.entityDoesNotExist <;> simp [h₄] at h₂
+    case ok edata =>
+      subst h₂
+      specialize h₁ edata
+      unfold PartialEntityData.ResidualsContainUnknowns at h₁
+      have h₅ := (Map.in_values_iff_findOrErr_ok (m := entities) (v := edata) (e := Error.entityDoesNotExist) wf).mpr
+      specialize h₅ (by exists uid)
+      exact h₁ h₅ rpval h₃
+  case h_3 => simp at h₂
 
 /--
   Inductive argument that partial evaluating a concrete `PartialExpr.getAttr`
@@ -97,18 +237,36 @@ theorem partial_eval_on_concrete_eqv_concrete_eval {x₁ : Expr} {request : Requ
   Inductive argument for `ResidualsContainUnknowns` for `PartialExpr.getAttr`
 -/
 theorem residuals_contain_unknowns {x₁ : PartialExpr} {request : PartialRequest} {entities : PartialEntities} {attr : String} :
-  @ResidualsContainUnknowns x₁ request entities →
-  @ResidualsContainUnknowns (PartialExpr.getAttr x₁ attr) request entities
+  entities.AllWellFormed →
+  @PartialExpr.ResidualsContainUnknowns x₁ request entities →
+  PartialEntities.ResidualsContainUnknowns entities →
+  @PartialExpr.ResidualsContainUnknowns (PartialExpr.getAttr x₁ attr) request entities
 := by
-  unfold ResidualsContainUnknowns
-  intro ih₁ r h₁
+  unfold PartialExpr.ResidualsContainUnknowns
+  intro wf ih₁ ih₂ r h₁
   unfold partialEvaluate at h₁
   cases h₂ : (partialEvaluate x₁ request entities) <;> simp [h₂] at h₁
   case ok pval₁ =>
     cases pval₁ <;> simp at h₁
     case value v₁ =>
-      -- need to argue that if `partialGetAttr` returns a residual, that residual contains an unknown
-      sorry
+      -- `v₁.attr` can return a residual even though `v₁` is concrete.
+      -- Here we argue that if it does, that residual contains an unknown
+      unfold partialGetAttr Except.map at h₁
+      split at h₁ <;> simp at h₁
+      case h_2 rpval h₃ =>
+        simp [RestrictedPartialValue.asPartialValue] at h₁
+        split at h₁ <;> simp at h₁
+        case h_2 r' =>
+          subst h₁
+          apply restrictedPartialExpr_to_PartialExpr_preserves_containsUnknown
+          cases h₄ : partialAttrsOf v₁ entities.attrs <;> simp [h₄] at h₃
+          case a.ok attrs =>
+            have h₅ := (Map.in_values_iff_findOrErr_ok (m := attrs) (v := .residual r') (e := Error.attrDoesNotExist) (partialAttrsOf_wf wf (partial_eval_wf wf h₂) h₄)).mpr
+            specialize h₅ (by exists attr)
+            unfold PartialEntities.AllWellFormed at wf
+            have h₆ := partialAttrsOf_ResidualsContainUnknowns wf.left ih₂ h₄ (.residual r')
+            simp [RestrictedPartialValue.ResidualsContainUnknowns] at h₆
+            exact h₆ h₅
     case residual r₁ =>
       subst h₁
       apply lhs_unknown
