cedar-lean/Cedar/Thm/PartialEval/Unary.lean
@@ -75,10 +75,10 @@ theorem partial_eval_on_concrete_eqv_concrete_eval {x₁ : Expr} {request : Requ
   Inductive argument for `ResidualsContainUnknowns` for `PartialExpr.unaryApp`
 -/
 theorem residuals_contain_unknowns {x₁ : PartialExpr} {request : PartialRequest} {entities : PartialEntities} {op : UnaryOp} :
-  @ResidualsContainUnknowns x₁ request entities →
-  @ResidualsContainUnknowns (PartialExpr.unaryApp op x₁) request entities
+  @PartialExpr.ResidualsContainUnknowns x₁ request entities →
+  @PartialExpr.ResidualsContainUnknowns (PartialExpr.unaryApp op x₁) request entities
 := by
-  unfold ResidualsContainUnknowns
+  unfold PartialExpr.ResidualsContainUnknowns
   intro ih₁ r h₁
   unfold partialEvaluate at h₁
   cases h₂ : (partialEvaluate x₁ request entities) <;> simp [h₂] at h₁
